starting relaxing conditions of restarts

Weidenbach_Book/CDCL_FW.thy
@@ -661,14 +661,14 @@ next
                 using RS(2) RS(3) by force
               hence "(\<lambda>p pa. skip_or_resolve p pa \<and> no_step backtrack p)\<^sup>*\<^sup>* T W"
                 proof -
-                  have "(\<exists>vr19 vr16 vr17 vr18. vr19 (vr16::'st) vr17 \<and> vr19\<^sup>*\<^sup>* vr17 vr18 
-                       \<and> \<not> vr19\<^sup>*\<^sup>* vr16 vr18) 
-                    \<or> \<not> (skip_or_resolve T U \<and> no_step backtrack T) 
-                    \<or> \<not> (\<lambda>uu uua. skip_or_resolve uu uua \<and> no_step backtrack uu)\<^sup>*\<^sup>* U W 
+                  have "(\<exists>vr19 vr16 vr17 vr18. vr19 (vr16::'st) vr17 \<and> vr19\<^sup>*\<^sup>* vr17 vr18
+                       \<and> \<not> vr19\<^sup>*\<^sup>* vr16 vr18)
+                    \<or> \<not> (skip_or_resolve T U \<and> no_step backtrack T)
+                    \<or> \<not> (\<lambda>uu uua. skip_or_resolve uu uua \<and> no_step backtrack uu)\<^sup>*\<^sup>* U W
                     \<or> (\<lambda>uu uua. skip_or_resolve uu uua \<and> no_step backtrack uu)\<^sup>*\<^sup>* T W"
                     by force
                   then show ?thesis
-                    by (metis (no_types) \<open>(\<lambda>S T. skip_or_resolve S T \<and> no_step backtrack S)\<^sup>*\<^sup>* U W\<close> 
+                    by (metis (no_types) \<open>(\<lambda>S T. skip_or_resolve S T \<and> no_step backtrack S)\<^sup>*\<^sup>* U W\<close>
                       \<open>skip_or_resolve T U \<and> no_step backtrack T\<close> f1)
                 qed
               hence "(\<lambda>p pa. skip_or_resolve p pa \<and> no_step backtrack p)\<^sup>*\<^sup>* S W"
@@ -3013,5 +3013,361 @@ next
   ultimately show ?s' unfolding full0_def by blast
 qed
 
+lemma full0_cdcl_s_full0_cdcl_fw:
+  assumes
+    "conflicting R = C_True" and
+    inv: "cdcl_all_inv_mes R"
+  shows "full0 cdcl_s R V \<longleftrightarrow> full0 cdcl_fw_s R V" (is "?s' \<longleftrightarrow> ?fw")
+  by (simp add: assms(1) full0_cdcl_s'_full0_cdcl_fw full0_cdcl_s_iff_full0_cdcl_s' inv)
 end
+
+subsection \<open>Adding Restarts\<close>
+locale cdcl_cw_ops_restart =
+  cdcl_cw_ops +
+  fixes f :: "nat \<Rightarrow> nat"
+  assumes "strict_mono f"
+begin
+lemma
+  assumes "mono (g:: nat \<Rightarrow> nat)"
+  shows "\<exists>m. g m > n"
+oops
+end
+
+locale cdcl\<^sub>N\<^sub>O\<^sub>T_increasing_restarts_ops =
+  restart_ops cdcl\<^sub>N\<^sub>O\<^sub>T restart for
+    restart :: "'st \<Rightarrow> 'st \<Rightarrow> bool" and
+    cdcl\<^sub>N\<^sub>O\<^sub>T :: "'st \<Rightarrow> 'st \<Rightarrow> bool" +
+  fixes
+    f :: "nat \<Rightarrow> nat" and
+    bound_inv :: "'bound \<Rightarrow> 'st \<Rightarrow> bool" and
+    \<mu> :: "'bound \<Rightarrow> 'st \<Rightarrow> nat" and
+    cdcl\<^sub>N\<^sub>O\<^sub>T_inv :: "'st \<Rightarrow> bool" and
+    \<mu>_bound :: "'bound \<Rightarrow> 'st \<Rightarrow> nat"
+  assumes
+    mono_f: "mono f" and
+    f_diverge: "\<And>n. \<exists>m. f m > n" and
+    bound_inv: "\<And>A S T. cdcl\<^sub>N\<^sub>O\<^sub>T_inv S \<Longrightarrow> bound_inv A S \<Longrightarrow> cdcl\<^sub>N\<^sub>O\<^sub>T S T \<Longrightarrow> bound_inv A T" and
+    cdcl\<^sub>N\<^sub>O\<^sub>T_measure: "\<And>A S T. cdcl\<^sub>N\<^sub>O\<^sub>T_inv S \<Longrightarrow> bound_inv A S \<Longrightarrow> cdcl\<^sub>N\<^sub>O\<^sub>T S T \<Longrightarrow> \<mu> A T < \<mu> A S" and
+    measure_bound2: "\<And>A T U. cdcl\<^sub>N\<^sub>O\<^sub>T_inv T \<Longrightarrow> bound_inv A T \<Longrightarrow> cdcl\<^sub>N\<^sub>O\<^sub>T\<^sup>*\<^sup>* T U
+       \<Longrightarrow> \<mu> A U \<le> \<mu>_bound A T" and
+    measure_bound4: "\<And>A T U. cdcl\<^sub>N\<^sub>O\<^sub>T_inv T \<Longrightarrow> bound_inv A T \<Longrightarrow> cdcl\<^sub>N\<^sub>O\<^sub>T\<^sup>*\<^sup>* T U
+       \<Longrightarrow> \<mu>_bound A U \<le> \<mu>_bound A T" and
+    cdcl\<^sub>N\<^sub>O\<^sub>T_restart_inv: "\<And>A U V. cdcl\<^sub>N\<^sub>O\<^sub>T_inv U \<Longrightarrow> restart U V \<Longrightarrow> bound_inv A U \<Longrightarrow> bound_inv A V" and
+    exists_bound: "\<And>R S. cdcl\<^sub>N\<^sub>O\<^sub>T_inv R \<Longrightarrow> restart R S \<Longrightarrow> \<exists>A. bound_inv A S" and
+    cdcl\<^sub>N\<^sub>O\<^sub>T_inv: "\<And>S T. cdcl\<^sub>N\<^sub>O\<^sub>T_inv S \<Longrightarrow> cdcl\<^sub>N\<^sub>O\<^sub>T S T \<Longrightarrow> cdcl\<^sub>N\<^sub>O\<^sub>T_inv T" and
+    cdcl\<^sub>N\<^sub>O\<^sub>T_inv_restart: "\<And>S T. cdcl\<^sub>N\<^sub>O\<^sub>T_inv S \<Longrightarrow> restart S T \<Longrightarrow> cdcl\<^sub>N\<^sub>O\<^sub>T_inv T"
+begin
+
+lemma strict_mono_ge_id: "strict_mono (g::nat \<Rightarrow> nat) \<Longrightarrow> g n \<ge> n"
+  unfolding strict_mono_def apply (induction n, simp)
+  by (metis Suc_leI diff_diff_cancel lessI less_imp_diff_less)
+
+lemma f_le_point: "f n = a \<Longrightarrow> \<forall>m\<le>n. f m \<le> a"
+  using mono_f unfolding mono_def by blast
+
+lemma cdcl\<^sub>N\<^sub>O\<^sub>T_cdcl\<^sub>N\<^sub>O\<^sub>T_inv:
+  assumes
+    "(cdcl\<^sub>N\<^sub>O\<^sub>T^^n) S T" and
+    "cdcl\<^sub>N\<^sub>O\<^sub>T_inv S"
+  shows "cdcl\<^sub>N\<^sub>O\<^sub>T_inv T"
+  using assms by (induction n arbitrary: T) (auto intro:bound_inv cdcl\<^sub>N\<^sub>O\<^sub>T_inv)
+
+lemma cdcl\<^sub>N\<^sub>O\<^sub>T_bound_inv:
+  assumes
+    "(cdcl\<^sub>N\<^sub>O\<^sub>T^^n) S T" and
+    "cdcl\<^sub>N\<^sub>O\<^sub>T_inv S"
+    "bound_inv A S"
+  shows "bound_inv A T"
+  using assms by (induction n arbitrary: T) (auto intro:bound_inv cdcl\<^sub>N\<^sub>O\<^sub>T_cdcl\<^sub>N\<^sub>O\<^sub>T_inv)
+
+lemma rtranclp_cdcl\<^sub>N\<^sub>O\<^sub>T_cdcl\<^sub>N\<^sub>O\<^sub>T_inv:
+  assumes
+    "cdcl\<^sub>N\<^sub>O\<^sub>T\<^sup>*\<^sup>* S T" and
+    "cdcl\<^sub>N\<^sub>O\<^sub>T_inv S"
+  shows "cdcl\<^sub>N\<^sub>O\<^sub>T_inv T"
+  using assms by induction (auto intro: cdcl\<^sub>N\<^sub>O\<^sub>T_inv)
+
+lemma rtranclp_cdcl\<^sub>N\<^sub>O\<^sub>T_bound_inv:
+  assumes
+    "cdcl\<^sub>N\<^sub>O\<^sub>T\<^sup>*\<^sup>* S T" and
+    "bound_inv A S" and
+    "cdcl\<^sub>N\<^sub>O\<^sub>T_inv S"
+  shows "bound_inv A T"
+  using assms by induction (auto intro:bound_inv rtranclp_cdcl\<^sub>N\<^sub>O\<^sub>T_cdcl\<^sub>N\<^sub>O\<^sub>T_inv)
+
+lemma cdcl\<^sub>N\<^sub>O\<^sub>T_comp_n_le:
+  assumes
+    "(cdcl\<^sub>N\<^sub>O\<^sub>T^^(Suc n)) S T" and
+    "bound_inv A S"
+    "cdcl\<^sub>N\<^sub>O\<^sub>T_inv S"
+  shows "\<mu> A T < \<mu> A S - n"
+  using assms
+proof (induction n arbitrary: T)
+  case 0
+  thus ?case using cdcl\<^sub>N\<^sub>O\<^sub>T_measure by auto
+next
+  case (Suc n) note IH =this(1)[OF _ this(3) this(4)] and S_T =this(2) and b_inv = this(3) and
+  c_inv = this(4)
+  obtain U :: 'st where S_U: "(cdcl\<^sub>N\<^sub>O\<^sub>T^^(Suc n)) S U" and U_T: "cdcl\<^sub>N\<^sub>O\<^sub>T U T" using S_T by auto
+  then have "\<mu> A U < \<mu> A S - n" using IH[of U] by simp
+  moreover
+    have "bound_inv A U"
+      using S_U b_inv  cdcl\<^sub>N\<^sub>O\<^sub>T_bound_inv c_inv by blast
+    hence "\<mu> A T < \<mu> A U" using cdcl\<^sub>N\<^sub>O\<^sub>T_measure[OF _ _ U_T] S_U c_inv cdcl\<^sub>N\<^sub>O\<^sub>T_cdcl\<^sub>N\<^sub>O\<^sub>T_inv by auto
+  ultimately show ?case by linarith
+qed
+
+lemma rtranclp_cdcl\<^sub>N\<^sub>O\<^sub>T_measure:
+  assumes
+    "cdcl\<^sub>N\<^sub>O\<^sub>T\<^sup>*\<^sup>* S T" and
+    "bound_inv A S" and
+    "cdcl\<^sub>N\<^sub>O\<^sub>T_inv S"
+  shows "\<mu> A T \<le> \<mu> A S"
+  using assms
+proof (induction rule: rtranclp_induct)
+  case base
+  thus ?case by auto
+next
+  case (step T U) note IH =this(3)[OF this(4) this(5)] and st =this(1) and cdcl\<^sub>N\<^sub>O\<^sub>T= this(2) and
+    b_inv = this(4) and c_inv = this(5)
+  have "bound_inv A T"
+    by (meson cdcl\<^sub>N\<^sub>O\<^sub>T_bound_inv rtranclp_imp_relpowp st step.prems)
+  moreover have "cdcl\<^sub>N\<^sub>O\<^sub>T_inv T"
+    using c_inv rtranclp_cdcl\<^sub>N\<^sub>O\<^sub>T_cdcl\<^sub>N\<^sub>O\<^sub>T_inv st by blast
+  ultimately have "\<mu> A U < \<mu> A T" using cdcl\<^sub>N\<^sub>O\<^sub>T_measure[OF _ _ cdcl\<^sub>N\<^sub>O\<^sub>T] by auto
+  thus ?case using IH by linarith
+qed
+
+lemma cdcl\<^sub>N\<^sub>O\<^sub>T_comp_bounded:
+  assumes
+    "bound_inv A S" and "cdcl\<^sub>N\<^sub>O\<^sub>T_inv S" and "m \<ge> 1+\<mu> A S"
+  shows "\<not>(cdcl\<^sub>N\<^sub>O\<^sub>T ^^ m) S T"
+  using assms cdcl\<^sub>N\<^sub>O\<^sub>T_comp_n_le[of "m-1" S T A] by fastforce
+
+text \<open>
+  \<^item> @{term "m \<ge> f (Suc n)"} ensure that at least one step has been done.\<close>
+inductive cdcl\<^sub>N\<^sub>O\<^sub>T_with_restart_stgy where
+restart_step: "(cdcl\<^sub>N\<^sub>O\<^sub>T^^m) S T \<Longrightarrow> m \<ge> f n \<Longrightarrow> restart T U
+  \<Longrightarrow> cdcl\<^sub>N\<^sub>O\<^sub>T_with_restart_stgy (S, n) (U, Suc n)" |
+restart_full: "full cdcl\<^sub>N\<^sub>O\<^sub>T S T \<Longrightarrow> cdcl\<^sub>N\<^sub>O\<^sub>T_with_restart_stgy (S, n) (T, Suc n)"
+
+lemmas cdcl\<^sub>N\<^sub>O\<^sub>T_with_restart_induct = cdcl\<^sub>N\<^sub>O\<^sub>T_with_restart_stgy.induct[split_format(complete),
+  OF cdcl\<^sub>N\<^sub>O\<^sub>T_increasing_restarts_ops_axioms]
+
+lemma cdcl\<^sub>N\<^sub>O\<^sub>T_with_restart_stgy_cdcl\<^sub>N\<^sub>O\<^sub>T_with_restarts:
+  "cdcl\<^sub>N\<^sub>O\<^sub>T_with_restart_stgy S T \<Longrightarrow> cdcl\<^sub>N\<^sub>O\<^sub>T_with_restarts\<^sup>*\<^sup>* (fst S) (fst T)"
+proof (induction rule: cdcl\<^sub>N\<^sub>O\<^sub>T_with_restart_stgy.induct)
+  case (restart_step m S T n U)
+  hence "cdcl\<^sub>N\<^sub>O\<^sub>T\<^sup>*\<^sup>* S T" by (meson relpowp_imp_rtranclp)
+  hence "cdcl\<^sub>N\<^sub>O\<^sub>T_with_restarts\<^sup>*\<^sup>* S T" using cdcl\<^sub>N\<^sub>O\<^sub>T_with_restarts.intros(1)
+    rtranclp_mono[of cdcl\<^sub>N\<^sub>O\<^sub>T cdcl\<^sub>N\<^sub>O\<^sub>T_with_restarts] by blast
+  moreover have "cdcl\<^sub>N\<^sub>O\<^sub>T_with_restarts T U" using \<open>restart T U\<close> cdcl\<^sub>N\<^sub>O\<^sub>T_with_restarts.intros(2) by blast
+  ultimately show ?case by auto
+next
+  case (restart_full S T)
+  hence "cdcl\<^sub>N\<^sub>O\<^sub>T\<^sup>*\<^sup>* S T" unfolding full_def by auto
+  thus ?case using cdcl\<^sub>N\<^sub>O\<^sub>T_with_restarts.intros(1)
+    rtranclp_mono[of cdcl\<^sub>N\<^sub>O\<^sub>T cdcl\<^sub>N\<^sub>O\<^sub>T_with_restarts] by auto
+qed
+
+lemma cdcl\<^sub>N\<^sub>O\<^sub>T_with_restart_bound_inv:
+  assumes
+    "cdcl\<^sub>N\<^sub>O\<^sub>T_with_restart_stgy S T" and
+    "bound_inv A (fst S)" and
+    "cdcl\<^sub>N\<^sub>O\<^sub>T_inv (fst S)"
+  shows "bound_inv A (fst T)"
+  using assms apply (induction rule: cdcl\<^sub>N\<^sub>O\<^sub>T_with_restart_stgy.induct)
+    prefer 2 apply (metis Nitpick.rtranclp_unfold fstI full_def rtranclp_cdcl\<^sub>N\<^sub>O\<^sub>T_bound_inv)
+  by (metis cdcl\<^sub>N\<^sub>O\<^sub>T_bound_inv cdcl\<^sub>N\<^sub>O\<^sub>T_cdcl\<^sub>N\<^sub>O\<^sub>T_inv cdcl\<^sub>N\<^sub>O\<^sub>T_restart_inv fst_conv)
+
+lemma cdcl\<^sub>N\<^sub>O\<^sub>T_with_restart_cdcl\<^sub>N\<^sub>O\<^sub>T_inv:
+  assumes
+    "cdcl\<^sub>N\<^sub>O\<^sub>T_with_restart_stgy S T" and
+    "cdcl\<^sub>N\<^sub>O\<^sub>T_inv (fst S)"
+  shows "cdcl\<^sub>N\<^sub>O\<^sub>T_inv (fst  T)"
+  using assms apply induction
+    apply (metis cdcl\<^sub>N\<^sub>O\<^sub>T_cdcl\<^sub>N\<^sub>O\<^sub>T_inv cdcl\<^sub>N\<^sub>O\<^sub>T_inv_restart fst_conv)
+   apply (metis fstI full0_def full0_unfold rtranclp_cdcl\<^sub>N\<^sub>O\<^sub>T_cdcl\<^sub>N\<^sub>O\<^sub>T_inv)
+  done
+
+lemma rtranclp_cdcl\<^sub>N\<^sub>O\<^sub>T_with_restart_cdcl\<^sub>N\<^sub>O\<^sub>T_inv:
+  assumes
+    "cdcl\<^sub>N\<^sub>O\<^sub>T_with_restart_stgy\<^sup>*\<^sup>* S T" and
+    "cdcl\<^sub>N\<^sub>O\<^sub>T_inv (fst S)"
+  shows "cdcl\<^sub>N\<^sub>O\<^sub>T_inv (fst T)"
+  using assms by induction (auto intro: cdcl\<^sub>N\<^sub>O\<^sub>T_with_restart_cdcl\<^sub>N\<^sub>O\<^sub>T_inv)
+
+lemma rtranclp_cdcl\<^sub>N\<^sub>O\<^sub>T_with_restart_bound_inv:
+  assumes
+    "cdcl\<^sub>N\<^sub>O\<^sub>T_with_restart_stgy\<^sup>*\<^sup>* S T" and
+    "cdcl\<^sub>N\<^sub>O\<^sub>T_inv (fst S)" and
+    "bound_inv A (fst S)"
+  shows "bound_inv A (fst T)"
+  using assms apply induction
+   apply (simp add: cdcl\<^sub>N\<^sub>O\<^sub>T_cdcl\<^sub>N\<^sub>O\<^sub>T_inv cdcl\<^sub>N\<^sub>O\<^sub>T_with_restart_bound_inv)
+  using cdcl\<^sub>N\<^sub>O\<^sub>T_with_restart_bound_inv rtranclp_cdcl\<^sub>N\<^sub>O\<^sub>T_with_restart_cdcl\<^sub>N\<^sub>O\<^sub>T_inv by blast
+
+lemma cdcl\<^sub>N\<^sub>O\<^sub>T_with_restart_increasing_number:
+  "cdcl\<^sub>N\<^sub>O\<^sub>T_with_restart_stgy S T \<Longrightarrow> snd T = 1 + snd S"
+  by (induction rule: cdcl\<^sub>N\<^sub>O\<^sub>T_with_restart_stgy.induct) auto
+end
+
+
+locale cdcl\<^sub>N\<^sub>O\<^sub>T_increasing_restarts =
+  cdcl\<^sub>N\<^sub>O\<^sub>T_increasing_restarts_ops restart cdcl\<^sub>N\<^sub>O\<^sub>T f bound_inv \<mu> cdcl\<^sub>N\<^sub>O\<^sub>T_inv \<mu>_bound
+  for
+    trail :: "'st \<Rightarrow> ('v, 'lvl, 'mark) annoted_lits" and
+    clauses :: "'st \<Rightarrow> 'v clauses" and
+    update_trail :: "('v, 'lvl, 'mark) annoted_lits \<Rightarrow> 'st \<Rightarrow> 'st" and
+    update_cls :: "'v clause set \<Rightarrow> 'st \<Rightarrow> 'st" and
+    f :: "nat \<Rightarrow> nat" and
+    restart :: "'st \<Rightarrow> 'st \<Rightarrow> bool" and
+    bound_inv :: "'bound \<Rightarrow> 'st \<Rightarrow> bool" and
+    \<mu> :: "'bound \<Rightarrow> 'st \<Rightarrow> nat" and
+    cdcl\<^sub>N\<^sub>O\<^sub>T :: "'st \<Rightarrow> 'st \<Rightarrow> bool" and
+    cdcl\<^sub>N\<^sub>O\<^sub>T_inv :: "'st \<Rightarrow> bool" and
+    \<mu>_bound :: "'bound \<Rightarrow> 'st \<Rightarrow> nat" +
+  assumes
+    measure_bound: "\<And>A T V n. cdcl\<^sub>N\<^sub>O\<^sub>T_inv T \<Longrightarrow> bound_inv A T
+      \<Longrightarrow> cdcl\<^sub>N\<^sub>O\<^sub>T_with_restart_stgy (T, n) (V, Suc n) \<Longrightarrow> \<mu> A V \<le> \<mu>_bound A T" and
+    cdcl\<^sub>N\<^sub>O\<^sub>T_with_restarts_\<mu>_bound:
+      "cdcl\<^sub>N\<^sub>O\<^sub>T_with_restart_stgy (T, a) (V, b) \<Longrightarrow>  cdcl\<^sub>N\<^sub>O\<^sub>T_inv T \<Longrightarrow> bound_inv A T
+        \<Longrightarrow> \<mu>_bound A V \<le> \<mu>_bound A T"
+begin
+
+lemma rtranclp_cdcl\<^sub>N\<^sub>O\<^sub>T_with_restarts_\<mu>_bound:
+  "cdcl\<^sub>N\<^sub>O\<^sub>T_with_restart_stgy\<^sup>*\<^sup>* (T, a) (V, b) \<Longrightarrow>  cdcl\<^sub>N\<^sub>O\<^sub>T_inv T \<Longrightarrow> bound_inv A T
+    \<Longrightarrow> \<mu>_bound A V \<le> \<mu>_bound A T"
+  apply (induction rule: rtranclp_induct2)
+   apply simp
+  by (metis cdcl\<^sub>N\<^sub>O\<^sub>T_with_restarts_\<mu>_bound dual_order.trans fst_conv
+    rtranclp_cdcl\<^sub>N\<^sub>O\<^sub>T_with_restart_bound_inv rtranclp_cdcl\<^sub>N\<^sub>O\<^sub>T_with_restart_cdcl\<^sub>N\<^sub>O\<^sub>T_inv)
+
+lemma cdcl\<^sub>N\<^sub>O\<^sub>T_with_restarts_measure_bound:
+  "cdcl\<^sub>N\<^sub>O\<^sub>T_with_restart_stgy (T, a) (V, b) \<Longrightarrow>  cdcl\<^sub>N\<^sub>O\<^sub>T_inv T \<Longrightarrow> bound_inv A T \<Longrightarrow> \<mu> A V \<le> \<mu>_bound A T"
+  apply (cases rule: cdcl\<^sub>N\<^sub>O\<^sub>T_with_restart_stgy.cases)
+     apply simp
+    using measure_bound relpowp_imp_rtranclp apply fastforce
+   by (metis full0_def full0_unfold measure_bound2 prod.inject)
+
+lemma rtranclp_cdcl\<^sub>N\<^sub>O\<^sub>T_with_restarts_measure_bound:
+  "cdcl\<^sub>N\<^sub>O\<^sub>T_with_restart_stgy\<^sup>*\<^sup>* (T, a) (V, b) \<Longrightarrow>  cdcl\<^sub>N\<^sub>O\<^sub>T_inv T \<Longrightarrow> bound_inv A T \<Longrightarrow> \<mu> A V \<le> \<mu>_bound A T"
+  apply (induction rule: rtranclp_induct2)
+    apply (simp add: measure_bound2)
+  by (metis dual_order.trans fst_conv measure_bound2 r_into_rtranclp rtranclp.rtrancl_refl
+    rtranclp_cdcl\<^sub>N\<^sub>O\<^sub>T_with_restart_bound_inv rtranclp_cdcl\<^sub>N\<^sub>O\<^sub>T_with_restart_cdcl\<^sub>N\<^sub>O\<^sub>T_inv
+    rtranclp_cdcl\<^sub>N\<^sub>O\<^sub>T_with_restarts_\<mu>_bound)
+
+lemma "wf {(T, S). cdcl\<^sub>N\<^sub>O\<^sub>T_with_restart_stgy S T \<and> cdcl\<^sub>N\<^sub>O\<^sub>T_inv (fst S)}" (is "wf ?A")
+proof (rule ccontr)
+  assume "\<not> ?thesis"
+  then obtain g where
+    g: "\<And>i. cdcl\<^sub>N\<^sub>O\<^sub>T_with_restart_stgy (g i) (g (Suc i))" and
+    cdcl\<^sub>N\<^sub>O\<^sub>T_inv_g: "\<And>i. cdcl\<^sub>N\<^sub>O\<^sub>T_inv (fst (g i))"
+    unfolding wf_iff_no_infinite_down_chain by fast
+  hence "\<And>i. snd (g i) < snd (g (i+1))"
+    by (metis Suc_eq_plus1 add.left_neutral add_Suc cdcl\<^sub>N\<^sub>O\<^sub>T_with_restart_increasing_number lessI)
+  have "strict_mono (snd o g)"
+    unfolding strict_mono_def by (smt Suc_eq_plus1 cdcl\<^sub>N\<^sub>O\<^sub>T_with_restart_increasing_number comp_def g
+      lessI lift_Suc_mono_less semiring_normalization_rules(24))
+  { fix i m
+    have "(cdcl\<^sub>N\<^sub>O\<^sub>T_with_restart_stgy^^m) (g i) (g (i+m))"
+      apply (induction m)
+       apply simp
+      using g[of "i+ _"] by auto
+    } note cdcl\<^sub>N\<^sub>O\<^sub>T_m = this
+  { fix i
+    have H: "\<And>T Ta m. (cdcl\<^sub>N\<^sub>O\<^sub>T ^^ m) T Ta \<Longrightarrow> no_step cdcl\<^sub>N\<^sub>O\<^sub>T T \<Longrightarrow> m = 0"
+      apply (case_tac m) apply simp by (meson relpowp_E2)
+    have "(cdcl\<^sub>N\<^sub>O\<^sub>T_with_restart_stgy^^(f (snd (g (i))))) (g i) (g (i+f (snd (g (i)))))"
+       using cdcl\<^sub>N\<^sub>O\<^sub>T_m by auto
+    have \<theta>: "\<And>S. \<exists>T m. (cdcl\<^sub>N\<^sub>O\<^sub>T ^^ m) S T"
+      by (meson relpowp_0_I)
+    have "\<exists> T m. (cdcl\<^sub>N\<^sub>O\<^sub>T ^^ m) (fst (g i)) T \<and> m \<ge> f (snd (g (i)))"
+      using g[of i] apply (cases rule: cdcl\<^sub>N\<^sub>O\<^sub>T_with_restart_stgy.cases)
+        apply auto[]
+      using g[of "Suc i"] apply (cases rule: cdcl\<^sub>N\<^sub>O\<^sub>T_with_restart_stgy.cases)
+      by (auto simp add: full_def full0_def \<theta> dest!: H f_le_point dest: tranclpD)
+  } note H = this
+  obtain m\<^sub>1 where "f m\<^sub>1 > 0" and [simp]: "m\<^sub>1 > 0"
+    using f_diverge by (metis less_irrefl_nat less_nat_zero_code not_gr0)
+  obtain A where "bound_inv A (fst (g m\<^sub>1))"
+    using g[of "m\<^sub>1-1"] cdcl\<^sub>N\<^sub>O\<^sub>T_inv_g g[of "m\<^sub>1"] \<open>m\<^sub>1 > 0\<close> \<open>f m\<^sub>1 > 0\<close> apply (cases rule: cdcl\<^sub>N\<^sub>O\<^sub>T_with_restart_stgy.cases)
+      apply (metis One_nat_def Suc_pred \<open>0 < m\<^sub>1\<close> cdcl\<^sub>N\<^sub>O\<^sub>T_cdcl\<^sub>N\<^sub>O\<^sub>T_inv exists_bound fst_conv)
+    apply (auto simp: cdcl\<^sub>N\<^sub>O\<^sub>T_with_restart_stgy.simps simp: full_def dest: tranclpD)
+    apply (subgoal_tac "f (Suc n) > 0")
+      apply (metis not_less relpowp_E2)
+      unfolding full_def sorry
+  let ?j = "\<mu>_bound A (fst (g m\<^sub>1)) + 1"
+  obtain m\<^sub>0 where "f m\<^sub>0 \<ge> ?j"
+    by (meson f_diverge linear not_less)
+  {
+     fix i j
+     have cdcl\<^sub>N\<^sub>O\<^sub>T_with_restart: "j \<ge> i \<Longrightarrow> cdcl\<^sub>N\<^sub>O\<^sub>T_with_restart_stgy\<^sup>*\<^sup>* (g i) (g j)"
+       apply (induction j)
+         apply simp
+       by (metis g le_Suc_eq rtranclp.rtrancl_into_rtrancl rtranclp.rtrancl_refl)
+  } note cdcl\<^sub>N\<^sub>O\<^sub>T_with_restart_stgy = this
+  have "cdcl\<^sub>N\<^sub>O\<^sub>T_inv (fst (g (Suc 0)))"
+    by (simp add: cdcl\<^sub>N\<^sub>O\<^sub>T_inv_g)
+  have "cdcl\<^sub>N\<^sub>O\<^sub>T_with_restart_stgy\<^sup>*\<^sup>*  (g m\<^sub>1) (g ?j)"
+    apply (rule cdcl\<^sub>N\<^sub>O\<^sub>T_with_restart_stgy)
+oops
+(*     sledgehammer
+    by (simp add: Suc_leI cdcl\<^sub>N\<^sub>O\<^sub>T_with_restart_stgy)
+  have "\<mu> A (fst (g ?j)) \<le> \<mu>_bound A (fst (g m\<^sub>1))"
+    apply (rule rtranclp_cdcl\<^sub>N\<^sub>O\<^sub>T_with_restarts_measure_bound)
+    using \<open>cdcl\<^sub>N\<^sub>O\<^sub>T_with_restart_stgy\<^sup>*\<^sup>* (fst (g m\<^sub>1), snd (g m\<^sub>1)) (fst (g ?j), snd (g ?j))\<close> apply blast
+        apply (simp add: cdcl\<^sub>N\<^sub>O\<^sub>T_inv_g)
+       using \<open>bound_inv A (fst (g m\<^sub>1))\<close> apply simp
+    done
+  hence "\<mu> A (fst (g ?j)) \<le> ?j"
+    by auto
+  have inv: "bound_inv A (fst (g ?j))"
+    using \<open>bound_inv A (fst (g 1))\<close> \<open>cdcl\<^sub>N\<^sub>O\<^sub>T_inv (fst (g (Suc 0)))\<close>
+    by (meson cdcl\<^sub>N\<^sub>O\<^sub>T_inv_g cdcl\<^sub>N\<^sub>O\<^sub>T_with_restart_stgy not_add_less2 not_less
+      rtranclp_cdcl\<^sub>N\<^sub>O\<^sub>T_with_restart_bound_inv)
+  obtain T m where
+    cdcl\<^sub>N\<^sub>O\<^sub>T_m: "(cdcl\<^sub>N\<^sub>O\<^sub>T ^^ m) (fst (g ?j)) T" and
+    f_m: "m\<^sub>0 \<le> m"
+    using H[of "?j"] by blast
+  have "?j \<le> m"
+    using f_m \<open>f m\<^sub>0 \<ge> ?j\<close> Nat.le_trans strict_mono_ge_id sorry
+  thus False
+    proof -
+      have "\<And>n. bound_inv A (fst (g (n + 1)))"
+        by (meson \<open>bound_inv A (fst (g 1))\<close> cdcl\<^sub>N\<^sub>O\<^sub>T_inv_g cdcl\<^sub>N\<^sub>O\<^sub>T_with_restart_stgy le_add2
+          rtranclp_cdcl\<^sub>N\<^sub>O\<^sub>T_with_restart_bound_inv)
+      moreover have "\<And>b. \<not> bound_inv b (fst (g (1 + \<mu>_bound A (fst (g 1)))))
+          \<or> \<not> 1 + \<mu> b (fst (g (1 + \<mu>_bound A (fst (g 1))))) \<le> m"
+        using cdcl\<^sub>N\<^sub>O\<^sub>T_comp_bounded cdcl\<^sub>N\<^sub>O\<^sub>T_inv_g cdcl\<^sub>N\<^sub>O\<^sub>T_m by force
+      ultimately show ?thesis
+        using \<open>\<mu> A (fst (g (\<mu>_bound A (fst (g 1)) + 1))) \<le> \<mu>_bound A (fst (g 1))\<close>
+        \<open>\<mu>_bound A (fst (g 1)) + 1 \<le> m\<close> by fastforce
+    qed
+qed
+ *)
+lemma cdcl\<^sub>N\<^sub>O\<^sub>T_with_restart_stgy_steps_bigger_than_bound:
+  assumes
+    "cdcl\<^sub>N\<^sub>O\<^sub>T_with_restart_stgy S T" and
+    "bound_inv A (fst S)" and
+    "cdcl\<^sub>N\<^sub>O\<^sub>T_inv (fst S)" and
+    "f (snd S) > \<mu>_bound A (fst S)"
+  shows "full cdcl\<^sub>N\<^sub>O\<^sub>T (fst S) (fst T)"
+  using assms
+proof (induction rule: cdcl\<^sub>N\<^sub>O\<^sub>T_with_restart_stgy.induct)
+  case restart_full
+  thus ?case by auto
+next
+  case (restart_step m S T n U) note st = this(1) and f = this(2) and bound_inv = this(4) and
+    cdcl\<^sub>N\<^sub>O\<^sub>T_inv =this(5) and \<mu> = this(6)
+  then obtain m' where m: "m = Suc m'" by (cases m) auto
+  have "\<mu> A S - m' = 0"
+    using f bound_inv cdcl\<^sub>N\<^sub>O\<^sub>T_inv \<mu> m rtranclp_cdcl\<^sub>N\<^sub>O\<^sub>T_with_restarts_measure_bound by fastforce
+  hence False using cdcl\<^sub>N\<^sub>O\<^sub>T_comp_n_le[of m' S T A] restart_step unfolding m by simp
+  thus ?case by fast
+qed
+
+end
+
 end
